proof/theories/Example_Ruleset.v
@@ -104,7 +104,8 @@ Definition fw_env : env :=
      e_map := fun _ => [];
      e_routes := []; e_rt := fun _ => [];
      e_ifaddr := (fun _ => []); e_ifaddr6 := (fun _ => []);
-     e_limit := fun _ => 0; e_quota := fun _ => 0; e_connlimit := fun _ => 0 |}.
+     e_limit := fun _ => 0; e_quota := fun _ => 0; e_connlimit := fun _ => 0;
+     e_ct := fun _ _ => [] |}.
 
 (** ** The chains, translated rule-for-rule from ruleset.nft. *)
 
